src/dafny/utils/DFS.dfy
@@ -1,0 +1,80 @@
+/*
+ * Copyright 2023 Franck Cassez
+ *
+ * Licensed under the Apache License, Version 2.0 (the "License"); you may
+ * not use this file except in compliance with the License. You may obtain
+ * a copy of the License at http://www.apache.org/licenses/LICENSE-2.0
+ *
+ * Unless required by applicable law or agreed to in writing, software dis-
+ * tributed under the License is distributed on an "AS IS" BASIS, WITHOUT
+ * WARRANTIES OR CONDITIONS OF ANY KIND, either express or implied. See the
+ * License for the specific language governing permissions and limitations
+ * under the License.
+ */
+
+include "./CFGraph.dfy"
+include "./EVMObject.dfy"
+include "./State.dfy"
+include "MiscTypes.dfy"
+
+/**
+  * Provides Depth-First-Search history.
+  */
+module DFS {
+
+  import opened CFGraph
+  import opened EVMObject
+  import opened State
+  import opened MiscTypes
+
+  /**  DFS current path history. */
+  datatype PathHistory =
+    PathHistory(seen: seq<CFGNode>, seenPCs: seq<nat>, path: seq<bool>, seenStates: map<AState, CFGNode>) {
+
+    /** The history should be well-formed  */
+    predicate IsConsistent(c: EVMObj, s: ValidState) {
+      && |seen| == |seenPCs| == |path| + 1
+      && s in seenStates
+      && (forall k:: 0 <= k < |seen| ==> seen[k].id == path[..k])
+      && (forall k:: 0 <= k < |seen| ==> seen[k].seg.Some?)
+      && (forall k:: k in seen && k.seg.Some? ==> k.seg.v < |c.xs|)
+      && (s.PC() == seenPCs[|seenPCs| - 1])
+      && (forall k:: 0 <= k < |seen| ==> seenPCs[k] == c.xs[seen[k].seg.v].StartAddress())
+      && (forall s:: s in seenStates && seenStates[s].seg.Some? ==> seenStates[s].seg.v < |c.xs|)
+    }
+  }
+
+  const DEFAULT_PATH_HISTORY :=
+    PathHistory([CFGNode([], Some(0))], [0], [], map[DEFAULT_VALIDSTATE := CFGNode([], Some(0))])
+
+  /** DFS entire search history. */
+  datatype DFSHistory =
+    DFSHistory(seenStates: map<AState, CFGNode>) {
+
+
+    /** The history should be well-formed  */
+    predicate IsConsistent(c: EVMObj, s: ValidState) {
+      && (forall s:: s in seenStates && seenStates[s].seg.Some? ==> seenStates[s].seg.v < |c.xs|)
+    }
+  }
+
+  const DEFAULT_DFS_HISTORY :=
+    DFSHistory(map[DEFAULT_VALIDSTATE := CFGNode([], Some(0))])
+
+
+  /**  CFG computation  */
+  //   datatype CFGComputation = CFGComputation(
+  //     grph: BoolCFGraph,
+  //     states:  map<AState, CFGNode>) {
+
+  //     function Graph(): BoolCFGraph {
+  //       grph
+  //     }
+
+  //     function States(): map<AState, CFGNode> {
+  //       states
+  //     }
+  //   }
+
+
+}
